translate function

pageTable.dfy
@@ -11,17 +11,19 @@ const levelSizes := [10, 10]
 const offset := 12
 const pageSize: addr := 0x0FFF
 const numVpns: addr := 0x0010_0000
-const numOffsets := 0x1000
+const numOffsets: addr := 0x1000
 const numVpnParts: addr := 0x0400
 var currPfn: addr
 
 predicate pageTableInvariant()
 reads this
 reads root
-{0 <= currPfn < numVpns &&
-root.Length == numVpns as int &&
+reads if (root.Length == numVpnParts as int) then set i | 0 <= i < numVpnParts && root[i].Some? :: root[i].arr else {}
+{0 < currPfn < numVpns &&
+root.Length == numVpnParts as int &&
 // all pageTables have exactly `numVpns` entries
-forall i : nat :: ((0 <= i < root.Length) ==> (root[i] == Nil || root[i].arr.Length == numVpnParts as int))
+(forall i : nat :: ((0 <= i < root.Length) ==> (root[i] == Nil || root[i].arr.Length == numVpnParts as int))) &&
+(currPfn != 0 ==> (forall i : nat :: ((0 <= i < root.Length && root[i].Some?) ==> (forall j : nat :: (0 <= j < root[i].arr.Length) ==> root[i].arr[j] < currPfn))))
 
 }
 
@@ -30,18 +32,18 @@ ensures pageTableInvariant()
 ensures fresh(root)
 {
 
-  root := new secondLevelPtr[numVpns];
+  root := new secondLevelPtr[numVpnParts];
 
   new;
 
-  assert(root.Length == numVpns as int);
-  for i := 0 to numVpns as int
-    invariant root.Length == numVpns as int
+  assert(root.Length == numVpnParts as int);
+  for i := 0 to numVpnParts as int
+    invariant root.Length == numVpnParts as int
     invariant 0 <= i <= root.Length
     invariant forall j: nat :: 0 <= j < i ==> root[j] == Nil
     invariant fresh(root){
     root[i] := Nil by {
-      assert(root.Length == numVpns as int);
+      assert(root.Length == numVpnParts as int);
 
     }
   }
@@ -58,6 +60,63 @@ requires 0 <= vpnPart2 < numVpnParts{
   var err := tryInsertMapping(vpnPart1, vpnPart2, pfn);
 
 }*/
+lemma bvLess(a: nat, b: nat)
+requires 0 <= a <= 0xFFFF_FFFF
+requires 0 <= b <= 0xFFFF_FFFF
+requires a < b
+//ensures a as bv32 < b as bv32
+{
+}
+
+lemma bvLessAddr(a: addr, b: addr)
+requires 0 <= a <= 0xFFFF_FFFF
+requires 0 <= b <= 0xFFFF_FFFF
+requires a < b
+//ensures a as bv32 < b as bv32
+{
+  var aNat := a as nat;
+  var bNat := b as nat;
+  //assert(aNat as bv32 < bNat as bv32) by {
+    //bvLess(aNat, bNat);
+  //}
+}
+
+method buildAddr(pfn: addr, offset: addr) 
+returns (a: addr)
+requires 0 <= pfn < numVpns
+requires 0 <= offset < numOffsets
+//ensures (a as bv32 & 0xFFF) == offset as bv32
+//ensures (a as bv32 >> 12) == pfn as bv32
+{
+  var mask1: bv32 := 0xF_FFFF;
+  var b1 := (pfn as bv32 & mask1);
+  //assert(b1 == pfn as bv32);
+  assert(b1 <= mask1);
+  //assert(b1 < 0x1 as bv32 << 20);
+  //assert(b1 <= 0xF_FFFF as bv32);
+
+  //assert(pfnBv < numVpns as bv32);
+  //assert(0x10_0000 == 1 as bv32 << 20 as bv6);
+  //assert(pfnBv < numVpns as bv21);
+  var shifted := (b1 << 12);
+  //assert(shifted >> 12 == b1);
+  //assert(shifted >> 32 == 0);
+  //assert(shifted >> 12 == pfnBv) by {
+  //}
+  //assert(shifted & 0xFFF == 0);
+  var b := (shifted | offset as bv32);
+  
+  //assert(b >> 12 == pfnBv) by {
+    //assert(offset as bv32 >> 12 == 0) by {
+      //assert(0 <= offset < 0xFFF);
+      //assert(0xFFF as bv32 == )
+  //}
+  //assert(b & 0x0FFF == offset as bv32);
+  return (b as addr);
+}
+function getOffset(a: addr): addr {
+  (a as bv32 & 0x0FFF as bv32) as addr
+}
 
 method getVpn(vaddr: addr) returns(vpn: addr)
 ensures 0 <= vpn < numVpns{
@@ -95,22 +154,40 @@ method tryInsertMapping(vpnPart1: addr, vpnPart2: addr, pfn: addr) returns (err:
 requires pageTableInvariant()
 requires 0 <= vpnPart1 < numVpnParts
 requires 0 <= vpnPart2 < numVpnParts
+requires pfn < currPfn
 ensures 0 <= err <= 1
 ensures pageTableInvariant()
 ensures err == 0 ==> root[vpnPart1].Some? && root[vpnPart1].arr[vpnPart2] == pfn
+ensures (err != 0 && old(root[vpnPart1].Some?)) ==> root[vpnPart1].Some? && root[vpnPart1].arr == old(root[vpnPart1].arr)
 modifies root
 modifies if root[vpnPart1].Some? then {root[vpnPart1].arr} else {}
 {
 assert(forall i : nat :: ((0 <= i < root.Length) ==> (root[i] == Nil || root[i].arr.Length == numVpnParts as int)));
+assert(forall i : nat :: ((0 <= i < root.Length && root[i].Some?) ==> (forall j :: (0 <= j < root[i].arr.Length) ==> root[i].arr[j] < currPfn)));
 
   var entry1 := root[vpnPart1];
 
   if (entry1 == Nil){
+assert(forall i : nat :: ((0 <= i < root.Length) ==> (root[i] == Nil || root[i].arr.Length == numVpnParts as int)));
     var a := new addr[numVpnParts];
+    for i := 0 to numVpnParts as int
+      invariant a.Length == numVpnParts as int
+      invariant 0 <= i <= a.Length
+      invariant forall j: nat :: 0 <= j < i ==> a[j] == 0 as addr
+      // these invariants are irrelevant to this loop but are necessary to prove later assertions
+      invariant forall i : nat :: ((0 <= i < root.Length) ==> (root[i] == Nil || root[i].arr.Length == numVpnParts as int))
+      invariant forall i : nat :: ((0 <= i < root.Length && root[i].Some?) ==> (forall j :: (0 <= j < root[i].arr.Length) ==> root[i].arr[j] < currPfn))
+      {
+      a[i] := 0 as addr by {
+        assert(a.Length == numVpnParts as int);
+
+      }
+    }
+    assert(forall i :: 0 <= i < a.Length ==> a[i] == 0 as addr);
+
     entry1 := Some(a);
     root[vpnPart1] := entry1;
     assert(entry1.arr.Length == numVpnParts as int);
-    entry1.arr[0] := 1;
   }
 
 
@@ -124,12 +201,22 @@ assert(forall i : nat :: ((0 <= i < root.Length) ==> (root[i] == Nil || root[i].
   if (entry2 == 0){
     entry2 := pfn;
     entry1.arr[vpnPart2] := entry2;
+    assert(entry2 < currPfn);
   }
   
 
   if (entry2 == pfn){
     // important assertions
-    var getPfn := tryGetMapping(vpnPart1, vpnPart2);
+    var getPfn := tryGetMapping(vpnPart1, vpnPart2) by {
+      assert(forall i : nat :: ((0 <= i < root.Length) ==> (root[i] == Nil || root[i].arr.Length == numVpnParts as int))) ;
+      assert(forall j :: 0 <= j < numVpnParts ==> root[vpnPart1].arr[j] < currPfn) by {
+        assert(root[vpnPart1].Some? && root[vpnPart1].arr[vpnPart2] == pfn);
+        assert(old(root[vpnPart1].Some?) ==> forall j :: 0 <= j < numVpnParts && j != vpnPart2 ==> root[vpnPart1].arr[j] == old(root[vpnPart1].arr[j]));
+        assert(old(root[vpnPart1].Some?) ==> forall j :: 0 <= j < numVpnParts && j != vpnPart2 ==> root[vpnPart1].arr[j] < currPfn);
+        assert(!old(root[vpnPart1].Some?) ==> forall j :: 0 <= j < numVpnParts && j != vpnPart2 ==> root[vpnPart1].arr[j] == 0);
+      }
+      assert(forall i : nat :: ((0 <= i < root.Length && root[i].Some?) ==> (forall j :: (0 <= j < root[i].arr.Length) ==> root[i].arr[j] < currPfn)));
+    }
     assert(pfn == getPfn);
     return 0;
   } else{
@@ -145,6 +232,7 @@ method tryGetMapping(vpnPart1: addr, vpnPart2: addr) returns (pfn: addr)
   requires pageTableInvariant()
 ensures pageTableInvariant()
 ensures root[vpnPart1].Some? ==> pfn == root[vpnPart1].arr[vpnPart2]
+ensures currPfn != 0 ==> 0 <= pfn < currPfn
 {
 
   var entry1 := root[vpnPart1];
@@ -184,11 +272,34 @@ modifies this{
   var vpn := getVpn(vaddr);
 
   var part1, part2 := maskVpn(vpn);
-  err := tryInsertMapping(part1, part2, currPfn);
+  currPfn := currPfn + 1;
+  err := tryInsertMapping(part1, part2, currPfn-1);
 }
 
-method translate(vaddr: addr) requires false{
+method translate(vaddr: addr) returns (paddr: addr)
+requires pageTableInvariant()
+ensures pageTableInvariant()
+modifies root
+modifies set i | 0 <= i < numVpnParts && root[i].Some? :: root[i].arr
+modifies this{
   // easy to implement, do later
+  var vpn := getVpn(vaddr);
+
+  var part1, part2 := maskVpn(vpn);
+  var pfn := tryGetMapping(part1, part2);
+
+  if (pfn == 0){
+    var err := allocate(vaddr, 1);
+    if (err != 0) {
+      return 0;
+    }
+
+  }
+  pfn := tryGetMapping(part1, part2);
+
+  var offset := getOffset(vaddr);
+  paddr := buildAddr(pfn, offset);
+
 }
 
 }
